L_{0}\left(x,y,t\right)=\frac{t-x}{y-x}
L_{1}\left(x,y,t\right)=\left(1-t\right)x+ty
L_{split}(t,k)=L_{0}(0,\frac{1}{k},\operatorname{mod}(t,\frac{1}{k}))
L_{index}(t,k)=\operatorname{floor}(kt)+1

a_{1}\left(t\right) = \left(\operatorname{sin}\left(2 \cdot \pi \cdot t\right) , \operatorname{cos}\left(2 \cdot \pi \cdot t\right)\right)
C_{Circle}\left(t\right)=a_{1}\left(t\right)
a_{2}\left(t , v , u\right) = v \cdot t + u \cdot \left(1 - t\right)
c_{connect}\left(t , v , u\right)=a_{2}\left(t , v , u\right)
a_{4}\left(t , n , i\right) = c_{connect}\left(t , C_{Circle}\left(i / n\right) , C_{Circle}\left(\operatorname{mod}\left(i + 1 , n\right) / n\right)\right)
a_{3}\left(t , n\right) = a_{4}\left(L_{split}\left(t, n\right) , n , L_{index}\left(t, n\right)\right)
P_{Polygon}\left(t , n\right)=a_{3}\left(t , n\right)
a_{7}\left(t , i , j\right) = P_{Polygon}\left(t , 3 \cdot i + j - 1\right) + \left(2 \cdot j - 4 , 2 \cdot i - 4\right)
a_{6}\left(t , i\right) = a_{7}\left(L_{split}\left(t, 3\right) , i , L_{index}\left(t, 3\right)\right)
a_{5}\left(t\right) = a_{6}\left(L_{split}\left(t, 3\right) , L_{index}\left(t, 3\right)\right)
a_{8}\left(t\right) = C_{Circle}\left(t\right) \cdot 5
a_{9}\left(t , k\right)=\left\{k=1:a_{5}\left(t\right),k=2:a_{8}\left(t\right)\right\}
D_{Drawing}\left(t\right)=a_{9}\left(L_{split}\left(t, 2\right) , L_{index}\left(t, 2\right)\right)
D_{Drawing}\left(t\right)
